Pauline.lean
@@ -1,2 +1,5 @@
 import Pauline.Notation
 import Pauline.Statics
+import Pauline.Dynamics
+import Pauline.Interp
+import Pauline.Tactic
