README.md
@@ -2,3 +2,9 @@ Pauline
 ---
 
 A formalization of (a subset of) SML semantics in Lean.
+
+Called "Pauline" because it sounds like a mashup of "Polly", the course mascot
+of [150](https://www.cs.cmu.edu/~15150/index.html) and "Lean".
+
+This is held together with zipties and hotglue. A lot of it would need to be
+re-written to get into a usable state.
